InferenceRule 작성

src/02-Introduction-to-Semantics/Lecture02.Meta.fst
@@ -17,28 +17,36 @@ type program_t = | Mkprogram: expression:expression_t -> program_t
 (* executing a program means evaluating the expression to an integer. *)
 assume val evaluate : expression_t -> int
 
-type execute_t = program_t -> int
-val execute : execute_t
 let execute (program:program_t) : int = evaluate program.expression
-
-
-
-
-
-
-
-
-
 
 
 (* An *operational semantics* describes how a program executes on an abstract machine. *)
 assume new 
 type abstract_machine_t : eqtype
 
-type operational_semantic_t = abstract_machine_t -> execute_t
+type singleton_t (#dom_t:Type) (unique_element:dom_t) = x:dom_t{x == unique_element}
+type operational_semantic_t = abstract_machine_t -> (singleton_t execute)
 
-(*
-A *small-step* operational semantics describes how such an execution proceeds in terms of successive reductions
-—here, of an expression—until we reach a value that represents the result of the computation. 
+(* A *small-step* operational semantics describes 
+   how such an execution proceeds in terms of successive reductions—here, of an expression—
+   until we reach a value that represents the result of the computation. 
 *)
+assume val reduced : expression_t -> expression_t -> prop
+
+let is_full_reduced (expression:expression_t) : prop = 
+   forall (x:expression_t). ~(expression `reduced` x)
+
+assume val cast_to_int : (expression:expression_t{is_full_reduced expression}) -> int
+
+type small_step_operational_semantic_t = (l:expression_t) -> (r:expression_t{l `reduced` r})
+
+assume val describe : 
+   (operational_semantic:operational_semantic_t) ->
+   (abstract_machine:abstract_machine_t) ->
+   (program:program_t) -> 
+   (x:list small_step_operational_semantic_t{
+      let result_value = operational_semantic abstract_machine program in
+      let result_expr = FStar.List.Tot.fold_left (fun e (s:small_step_operational_semantic_t) -> s e) program.expression x in
+      (is_full_reduced result_expr) /\ (cast_to_int result_expr = result_value)
+   })
 
