src/02-Introduction-to-Semantics/Lecture02.InferenceRule.fst
@@ -1,0 +1,23 @@
+module Lecture02.InferenceRule
+module L = FStar.List.Tot
+
+(* The small‑step operational semantics itself is a relation on configurations—i.e., a subset of Config × Config
+   Question: How should we define this relation? Remember that there are an infinite number of configurations and possible steps!
+   Answer: Define it inductively, using inference rules:
+
+   An inference rule defines an implication: if all the premises hold, then the conclusion also holds.
+*)
+
+noeq
+type t = {
+  #label_t: eqtype;
+  label: label_t;
+  model_t: Type;
+  premises: list (model_t -> prop);
+  conclusion: (model_t -> prop);
+}
+
+let is_example (rule:t) (model:rule.model_t) : prop =
+  (L.for_allP (fun premise -> premise model) rule.premises) ==> (rule.conclusion model)
+
+let is_valid (rule:t) : prop = forall (model:rule.model_t). (is_example rule model)
