src/common/Nemonuri.Unique.fst
@@ -5,6 +5,7 @@ module Nemonuri.Unique
    - https://en.wikipedia.org/wiki/Uniqueness_quantification
 *)
 
+
 let is_unique_element (#dom_t:eqtype) (predicate:dom_t -> prop) (elt:dom_t) : prop =
   (predicate elt) /\ (forall (y:dom_t). (predicate y) <==> (y = elt))
 
@@ -17,3 +18,4 @@ type singleton_predicate_t (dom_t:eqtype) = p:(dom_t -> prop){is_singleton_predi
 let get_unique_element #dom_t (singleton_predicate:singleton_predicate_t dom_t)
   : GTot (x:dom_t{is_unique_element singleton_predicate x}) =
   FStar.IndefiniteDescription.indefinite_description_ghost dom_t singleton_predicate
+
